theories/typing/lib/list.v
@@ -17,6 +17,10 @@ Section list.
     move=> ?. apply fix_leak=> ??. eapply leak_impl; [solve_typing|]. by case.
   Qed.
 
+  Lemma list_leak_just {𝔄} E L (ty: _ 𝔄) :
+    leak E L ty (const True) → leak E L (list_ty ty) (const True).
+  Proof. move=> ?. apply leak_just. Qed.
+
   Lemma list_subtype {𝔄 𝔅} E L (f: 𝔄 → 𝔅) ty ty' :
     subtype E L ty ty' f → subtype E L (list_ty ty) (list_ty ty') (map f).
   Proof.
@@ -30,4 +34,5 @@ Section list.
 
 End list.
 
-Global Hint Resolve list_leak list_subtype list_eqtype : lrust_typing.
+Global Hint Resolve list_leak | 5 : lrust_typing.
+Global Hint Resolve list_leak_just list_subtype list_eqtype : lrust_typing.
